simulate: make some progress on the static-call instruction

examples/custom/let_mut.rs
@@ -1,0 +1,13 @@
+fn let_mut() -> i32 {
+  let mut x = 5;
+  x = x + 1;
+  x
+}
+
+fn match_mut() -> i32 {
+  let Some(mut x) = Some(5) else {
+    return 0;
+  };
+  x = x + 1;
+  x
+}
