RocqOfRust/revm/revm_interpreter/instructions/simulate/contract/static_call.v
@@ -1,40 +1,62 @@
 Require Import RocqOfRust.RocqOfRust.
 Require Import RocqOfRust.links.M.
 Require Import RocqOfRust.simulate.M.
+Require Import alloy_primitives.bits.simulate.address.
+Require Import alloy_primitives.bits.simulate.fixed.
+Require Import core.links.array.
+Require Import core.simulate.result.
 Require Import revm.revm_context_interface.links.host.
+Require Import revm.revm_context_interface.simalte.host.
+Require Import revm.revm_interpreter.instructions.contract.simulate.call_helpers.
 Require Import revm.revm_interpreter.instructions.links.contract.static_call.
+Require Import revm.revm_interpreter.instructions.simulate.macros.
 Require Import revm.revm_interpreter.links.interpreter.
 Require Import revm.revm_interpreter.links.interpreter_types.
 Require Import revm.revm_interpreter.simulate.interpreter_types.
 Require Import revm.revm_specification.links.hardfork.
 Require Import revm.revm_specification.simulate.hardfork.
+Require Import ruint.simulate.from.
 
-Definition check_macro {WIRE : Set} `{Link WIRE}
+Definition static_call
+    {WIRE H : Set} `{Link WIRE} `{Link H}
     {WIRE_types : InterpreterTypes.Types.t} `{InterpreterTypes.Types.AreLinks WIRE_types}
     {IInterpreterTypes : InterpreterTypes.C WIRE_types}
+    {IHost : Host.C H}
     (interpreter : Interpreter.t WIRE WIRE_types)
-    (min : SpecId.t)
-    (k : Interpreter.t WIRE WIRE_types -> Interpreter.t WIRE WIRE_types) :
-    Interpreter.t WIRE WIRE_types :=
-  if
-    Impl_SpecId.is_enabled_in
-      (IInterpreterTypes
-          .(InterpreterTypes.RuntimeFlag)
-          .(SRuntimeFlag.spec_id)
-        interpreter.(Interpreter.runtime_flag)
-      )
-      min
-  then
-    k interpreter
-  else
+    (host : H) :
+    Interpreter.t WIRE WIRE_types * H :=
+  let inject_interpreter interpreter := (interpreter, host) in
+
+  check_macro interpreter SpecId.BYZANTIUM inject_interpreter (fun interpreter =>
+  popn_macro interpreter {| Integer.value := 2 |} inject_interpreter (fun arr interpreter =>
+  let '(_, to, local_gas_limit) := ArrayPairs.to_tuple_rev (arr.(array.value)) in
+  let to := Impl_Address.from_word (Impl_From_U256_for_FixedBytes_32.from to) in
+
+  let local_gas_limit :=
+    Impl_Result_T_E.unwrap_or
+      (TryFrom_Uint_for_u64.try_from local_gas_limit)
+      {| Integer.value := 2 ^ 64 - 1 |} in
+
+  match get_memory_input_and_out_ranges interpreter with
+  | (None, interpreter) => (interpreter, host)
+  | (Some (input, return_memory_offset), interpreter) =>
+
+  match IHost.(Host.load_account_delegated) host to with
+  | (None, host) =>
     let control :=
       IInterpreterTypes
           .(InterpreterTypes.Loop)
           .(Loop.set_instruction_result)
         interpreter.(Interpreter.control)
-        instruction_result.InstructionResult.NotActivated in
-    interpreter
-      <| Interpreter.control := control |>.
+        instruction_result.InstructionResult.FatalExternalError in
+    let interpreter :=
+      interpreter
+        <| Interpreter.control := control |> in
+    (interpreter, host)
+  | (Some load, host) =>
+
+  (interpreter, host)
+  end end)).
 
 Lemma static_call_eq
     {WIRE H : Set} `{Link WIRE} `{Link H}
@@ -45,6 +67,8 @@ Lemma static_call_eq
     (IInterpreterTypes : InterpreterTypes.C WIRE_types)
     (InterpreterTypesEq :
       InterpreterTypes.Eq.t WIRE WIRE_types run_InterpreterTypes_for_WIRE IInterpreterTypes)
+    (IHost : Host.C H)
+    (HostEq : Host.Eq.t run_Host_for_H IHost)
     (interpreter : Interpreter.t WIRE WIRE_types)
     (host : H) :
   let ref_interpreter := make_ref 0 in
@@ -57,42 +81,60 @@ Lemma static_call_eq
       [interpreter; host]%stack 🌲
     (
       Output.Success tt,
-      [
-        check_macro interpreter SpecId.BYZANTIUM (fun interpreter =>
-          interpreter
-        );
-        host
-      ]%stack
+      let (interpreter, host) := static_call interpreter host in
+      [interpreter; host]%stack
     )
   }}.
 Proof.
   intros.
   destruct InterpreterTypesEq as [[] [] []].
-  unfold run_static_call; cbn.
-  unfold check_macro; cbn.
+  destruct HostEq as [].
+  unfold run_static_call, static_call; cbn.
+  check_macro_eq spec_id set_instruction_result.
+  popn_macro_eq H IInterpreterTypes popn set_instruction_result.
   eapply Run.Call. {
-    apply spec_id.
+    apply Impl_From_U256_for_FixedBytes_32.from_eq.
   }
-  cbn.
   eapply Run.Call. {
-    apply Impl_SpecId.is_enabled_in_eq.
+    apply Impl_Address.from_word_eq.
   }
-  cbn.
   eapply Run.Call. {
-    apply Run.Pure.
+    apply TryFrom_Uint_for_u64.try_from_eq.
   }
-  cbn.
   eapply Run.Call. {
-    apply Run.Pure.
-  }
-  cbn.
-  destruct Impl_SpecId.is_enabled_in; cbn.
-  { admit. }
-  { eapply Run.Call. {
-      apply (set_instruction_result _ _ instruction_result.InstructionResult.NotActivated).
-    }
     cbn.
+    (* TODO: simulate the integer *)
+    eapply Run.Call. {
+      apply Run.Pure.
+    }
     apply Run.Pure.
   }
+  eapply Run.Call. {
+    apply Impl_Result_T_E.unwrap_or_eq.
+  }
+  eapply Run.Call. {
+    apply get_memory_input_and_out_ranges_eq.
+  }
+  cbn; fold @SimulateM.let_.
+  destruct get_memory_input_and_out_ranges as [[[input return_memory_offset]|] ?interpreter];
+    cbn;
+    [| apply Run.Pure].
+  get_can_access.
+  eapply Run.Call. {
+    apply load_account_delegated.
+  }
+  destruct IHost.(Host.load_account_delegated) as [[load|] ?host].
+  2: {
+    eapply Run.Call; [
+      apply (set_instruction_result
+        _
+        _
+        instruction_result.InstructionResult.FatalExternalError
+      )
+    |];
+    apply Run.Pure.
+  }
+  cbn.
+  get_can_access.
 Admitted.
 Global Opaque run_static_call.
