RocqOfRust/core/simulate/result.v
@@ -1,0 +1,33 @@
+Require Import RocqOfRust.RocqOfRust.
+Require Import RocqOfRust.links.M.
+Require Import RocqOfRust.simulate.M.
+Require Import core.links.result.
+
+Module Impl_Result_T_E.
+  Definition Self (T E : Set) : Set :=
+    Result.t T E.
+
+  Definition unwrap_or {T E : Set} (self : Self T E) (default : T) : T :=
+    match self with
+    | Result.Ok x => x
+    | Result.Err _ => default
+    end.
+
+  Lemma unwrap_or_eq {T E : Set} `{Link T} `{Link E} (stack : Stack.t)
+      (self : Self T E) (default : T) :
+    {{
+      SimulateM.eval_f (
+        result.Impl_Result_T_E.run_unwrap_or T E self default
+      )
+      stack 🌲
+      (
+        Output.Success (unwrap_or self default),
+        stack
+      )
+    }}.
+  Proof.
+    unfold run_unwrap_or; cbn.
+    destruct self; cbn; apply Run.Pure.
+  Qed.
+  Global Opaque run_unwrap_or.
+End Impl_Result_T_E.
