RocqOfRust/revm/revm_context_interface/simalte/host.v
@@ -1,0 +1,48 @@
+Require Import RocqOfRust.RocqOfRust.
+Require Import RocqOfRust.links.M.
+Require Import RocqOfRust.simulate.M.
+Require Import alloy_primitives.bits.links.address.
+Require Import revm.revm_context_interface.links.host.
+Require Import revm.revm_context_interface.links.journaled_state.
+
+Module Host.
+  Class C
+      (Self : Set) `{Link Self} :
+      Type := {
+    (* fn load_account_delegated(&mut self, address: Address) -> Option<AccountLoad>; *)
+    load_account_delegated :
+      forall
+        (self : Self)
+        (address : Address.t),
+      option AccountLoad.t *
+      Self;
+  }.
+
+  Module Eq.
+    Class t
+        {Self : Set} `{Link Self}
+        {types : Host.Types.t} `{Host.Types.AreLinks types}
+        (run_Host_for_Self : Host.Run Self types)
+        (I : C Self) :
+        Prop := {
+      load_account_delegated
+          {Interpreter : Set}
+          (interpreter : Interpreter)
+          (self : Self)
+          (address : Address.t)
+          (stack : Stack.t) :
+        let ref_self : Ref.t Pointer.Kind.MutRef Self := make_ref 1 in
+        {{
+          SimulateM.eval_f
+            (run_Host_for_Self.(links.host.Host.load_account_delegated).(TraitMethod.run)
+              ref_self address)
+            (interpreter :: self :: stack)%stack 🌲
+          let result_self := I.(load_account_delegated) self address in
+          (
+            Output.Success (fst result_self),
+            (interpreter :: snd result_self :: stack)%stack
+          )
+        }}
+    }.
+    End Eq.
+End Host.
