RocqOfRust/revm/revm_interpreter/instructions/simulate/macros.v
@@ -1,0 +1,229 @@
+Require Import RocqOfRust.RocqOfRust.
+Require Import RocqOfRust.links.M.
+Require Import RocqOfRust.simulate.M.
+Require Import alloy_primitives.links.aliases.
+Require Import revm.revm_interpreter.links.interpreter.
+Require Import revm.revm_interpreter.links.interpreter_types.
+Require Import revm.revm_interpreter.simulate.gas.
+Require Import revm.revm_interpreter.simulate.interpreter_types.
+Require Import revm.revm_specification.links.hardfork.
+Require Import revm.revm_specification.simulate.hardfork.
+
+Definition gas_macro {WIRE K : Set} `{Link WIRE}
+    {WIRE_types : InterpreterTypes.Types.t} `{InterpreterTypes.Types.AreLinks WIRE_types}
+    {IInterpreterTypes : InterpreterTypes.C WIRE_types}
+    (interpreter : Interpreter.t WIRE WIRE_types)
+    (cost : U64.t)
+    (k_exit : Interpreter.t WIRE WIRE_types -> K)
+    (k : Interpreter.t WIRE WIRE_types -> K) :
+    K :=
+  let gas :=
+    IInterpreterTypes
+        .(InterpreterTypes.Loop)
+        .(Loop.gas)
+        .(RefStub.projection)
+      interpreter.(Interpreter.control) in
+  match Impl_Gas.record_cost gas cost with
+  | None =>
+    let control :=
+      IInterpreterTypes
+          .(InterpreterTypes.Loop)
+          .(Loop.set_instruction_result)
+        interpreter.(Interpreter.control)
+        instruction_result.InstructionResult.OutOfGas in
+    let interpreter := interpreter
+      <| Interpreter.control := control |> in
+    k_exit interpreter
+  | Some gas =>
+    let control :=
+      IInterpreterTypes
+          .(InterpreterTypes.Loop)
+          .(Loop.gas)
+          .(RefStub.injection)
+        interpreter.(Interpreter.control) gas in
+    let interpreter :=
+      interpreter
+        <| Interpreter.control := control |> in
+    k interpreter
+  end.
+
+Ltac gas_macro_eq H gas set_instruction_result :=
+  unfold gas_macro;
+  eapply Run.Call; [
+    apply gas
+  |];
+  eapply Run.Call; [
+    apply Run.Pure
+  |];
+  eapply Run.Call; [
+    apply Impl_Gas.record_cost_eq
+  |];
+  destruct Impl_Gas.record_cost;
+  (
+    eapply Run.Call; [
+      apply Run.Pure
+    |]
+  );
+  [|
+    eapply Run.Call; [
+      apply Run.Pure
+    |];
+    eapply Run.Call; [
+      apply (set_instruction_result _ _ instruction_result.InstructionResult.OutOfGas)
+    |];
+    apply Run.Pure
+  ].
+
+Definition popn_macro {WIRE K : Set} `{Link WIRE}
+    {WIRE_types : InterpreterTypes.Types.t} `{InterpreterTypes.Types.AreLinks WIRE_types}
+    {IInterpreterTypes : InterpreterTypes.C WIRE_types}
+    (interpreter : Interpreter.t WIRE WIRE_types)
+    (N : Usize.t)
+    (k_exit : Interpreter.t WIRE WIRE_types -> K)
+    (k : array.t aliases.U256.t N -> Interpreter.t WIRE WIRE_types -> K) :
+    K :=
+    let stack := interpreter.(Interpreter.stack) in
+    let (result, stack) :=
+      IInterpreterTypes.(InterpreterTypes.Stack).(Stack.popn) N stack in
+    let interpreter :=
+      interpreter
+        <| Interpreter.stack := stack |> in
+    match result with
+    | Some arr => k arr interpreter
+    | None =>
+      let control :=
+        IInterpreterTypes.(InterpreterTypes.Loop).(Loop.set_instruction_result)
+        interpreter.(Interpreter.control)
+        instruction_result.InstructionResult.StackUnderflow in
+      let interpreter := interpreter
+        <| Interpreter.control := control |> in
+      k_exit interpreter
+    end.
+
+Ltac popn_macro_eq H IInterpreterTypes popn set_instruction_result :=
+  unfold popn_macro;
+  eapply Run.Call; [
+    apply popn
+  |];
+  destruct IInterpreterTypes.(InterpreterTypes.Stack).(Stack.popn) as [[|] ?]; cbn; [|
+    eapply Run.Call; [
+      apply (set_instruction_result
+        _
+        _
+        instruction_result.InstructionResult.StackUnderflow
+      )
+    |];
+    cbn;
+    apply Run.Pure
+  ].
+
+Definition popn_top_macro {WIRE K : Set} `{Link WIRE}
+    {WIRE_types : InterpreterTypes.Types.t} `{InterpreterTypes.Types.AreLinks WIRE_types}
+    {IInterpreterTypes : InterpreterTypes.C WIRE_types}
+    (interpreter : Interpreter.t WIRE WIRE_types)
+    (N : Usize.t)
+    (k_exit : Interpreter.t WIRE WIRE_types -> K)
+    (k :
+      array.t aliases.U256.t N ->
+      RefStub.t WIRE_types.(InterpreterTypes.Types.Stack) aliases.U256.t ->
+      Interpreter.t WIRE WIRE_types ->
+      K
+    ) :
+    K :=
+  let stack := interpreter.(Interpreter.stack) in
+  let (result, stack) :=
+    IInterpreterTypes
+        .(InterpreterTypes.Stack)
+        .(Stack.popn_top)
+      N stack in
+  let interpreter :=
+    interpreter
+      <| Interpreter.stack := stack |> in
+  match result with
+  | Some (arr, top) =>
+    k arr top interpreter
+  | None =>
+    let control :=
+      IInterpreterTypes.(InterpreterTypes.Loop).(Loop.set_instruction_result)
+        interpreter.(Interpreter.control)
+        instruction_result.InstructionResult.StackUnderflow in
+    let interpreter := interpreter
+      <| Interpreter.control := control |> in
+    k_exit interpreter
+  end.
+
+Ltac popn_top_macro_eq H IInterpreterTypes popn_top set_instruction_result :=
+  unfold popn_top_macro;
+  eapply Run.Call; [
+    apply Run.Pure
+  |];
+  eapply Run.Call; [
+    apply popn_top
+  |];
+  destruct IInterpreterTypes.(InterpreterTypes.Stack).(Stack.popn_top) as [[[? ?]|] ?];
+  [|
+    eapply Run.Call; [
+      apply (set_instruction_result
+        _
+        _
+        instruction_result.InstructionResult.StackUnderflow
+      )
+    |];
+    apply Run.Pure
+  ].
+
+Definition check_macro {WIRE K : Set} `{Link WIRE}
+    {WIRE_types : InterpreterTypes.Types.t} `{InterpreterTypes.Types.AreLinks WIRE_types}
+    {IInterpreterTypes : InterpreterTypes.C WIRE_types}
+    (interpreter : Interpreter.t WIRE WIRE_types)
+    (min : SpecId.t)
+    (k_exit : Interpreter.t WIRE WIRE_types -> K)
+    (k : Interpreter.t WIRE WIRE_types -> K) :
+    K :=
+  if
+    Impl_SpecId.is_enabled_in
+      (IInterpreterTypes
+          .(InterpreterTypes.RuntimeFlag)
+          .(SRuntimeFlag.spec_id)
+        interpreter.(Interpreter.runtime_flag)
+      )
+      min
+  then
+    k interpreter
+  else
+    let control :=
+      IInterpreterTypes
+          .(InterpreterTypes.Loop)
+          .(Loop.set_instruction_result)
+        interpreter.(Interpreter.control)
+        instruction_result.InstructionResult.NotActivated in
+    let interpreter :=
+      interpreter
+        <| Interpreter.control := control |> in
+    k_exit interpreter.
+
+Ltac check_macro_eq spec_id set_instruction_result :=
+  unfold check_macro; cbn;
+  eapply Run.Call; [
+    apply spec_id
+  |];
+  cbn;
+  eapply Run.Call; [
+    apply Impl_SpecId.is_enabled_in_eq
+  |];
+  cbn;
+  eapply Run.Call; [
+    apply Run.Pure
+  |];
+  cbn;
+  eapply Run.Call; [
+    apply Run.Pure
+  |];
+  cbn;
+  destruct Impl_SpecId.is_enabled_in; cbn; [|
+    eapply Run.Call; [
+      apply (set_instruction_result _ _ instruction_result.InstructionResult.NotActivated)
+    |];
+    cbn;
+    apply Run.Pure
+  ].
